@prefix cc: <http://creativecommons.org/ns#> .
@prefix dc: <http://purl.org/dc/elements/1.1/> .
@prefix owl: <http://www.w3.org/2002/07/owl#> .
@prefix rdf: <http://www.w3.org/1999/02/22-rdf-syntax-ns#> .
@prefix xml: <http://www.w3.org/XML/1998/namespace> .
@prefix xsd: <http://www.w3.org/2001/XMLSchema#> .
@prefix rdfs: <http://www.w3.org/2000/01/rdf-schema#> .
@prefix schema: <http://schema.org/> . 
@prefix foaf: <http://xmlns.com/foaf/0.1/> .
@prefix obo: <http://purl.obolibrary.org/obo/> .
@prefix p: <http://dbpedia.org/resource/> .
@prefix kb:<http://kbpedia.org/kko/rc/> .
@prefix dbo: <http://dbpedia.org/ontology/> .
@prefix vcard: <http://www.w3.org/2006/vcard/ns#>  .
@prefix dct:     <http://purl.org/dc/terms/> .

@prefix lexlegal: <http://linkedopendatang.com/schemas/lexanalytics/lexanalytics-owl.ttl#> .
@prefix lexvocab: <http://linkedopendatang.com/schemas/lexanalytics/lexanalytics-skos-vocab#> .
@prefix ngconstitution: <http://www.constituteproject.org/constitution/Nigeria_2011/> .



<http://linkedopendatang.com/schemas/lexanalytics/lexanalytics-owl.ttl>
  cc:license <http://creativecommons.org/licenses/by-sa/3.0/> ;
  rdf:type owl:Ontology ;
  rdfs:label "Lexanalytic Ontology for Nigerian Legal data" ;
  dc:date "2020-10-01"^^xsd:date ;
  dct:description "This is a document that uses Linked Data oriented content to describe an Ontology for Lexanalytics. It is a data model for publishing legal data as a Graph. This is an evolving spec." ;
  owl:versionInfo "0.1.0" ;
  dct:title "Lexanalytics Ontology";
  dct:created "2020-10-01"^^xsd:date;
  dct:modified "2020-12-19"^^xsd:date;
  dct:modified "2022-05-26"^^xsd:date;

  foaf:maker <http://twitter.com/emekaokoye#this> .
  

<http://www.constituteproject.org/constitution/Nigeria_2011/>  
  a lexlegal:Constitution ;
  rdfs:label "2011 Nigerian Constitution" .

# ---------------------------------------------------------------------------
# CLASSES
#


lexlegal:Object
    a owl:Class;
	dc:identifier "Object" ;
    rdfs:isDefinedBy lexlegal: ;
    rdfs:label "LexanalyticsObject" ;
    rdfs:comment "A base class representing all Lexanalytics objects" .

	
lexlegal:Person
    a owl:Class ;
    rdfs:subClassOf lexlegal:Object ;
    rdfs:subClassOf schema:Person;
    rdfs:subClassOf foaf:Person;
    rdfs:isDefinedBy lexlegal: ;
    rdfs:label "Person" ;
	dct:description "A human being regarded as an individual." ;
	dc:identifier "Person" ;
    rdfs:comment "A class representing a Person" .

	
lexlegal:Document
    a owl:Class ;
    rdfs:subClassOf lexlegal:Object;
    rdfs:subClassOf foaf:Document;
    rdfs:isDefinedBy lexlegal: ;
    rdfs:label "Document" ;
	dc:identifier "Document" ;
	dct:description "A piece of written, printed, or electronic matter that provides information or evidence or that serves as an official record" ;
    rdfs:comment "A class representing a Document" .

    
lexlegal:Case
    a owl:Class ;    
    rdfs:subClassOf lexlegal:Document;
    rdfs:isDefinedBy lexlegal: ;
    rdfs:label "Case" ;
 	dc:identifier "Case" ;
	dct:description "A legal action, especially one to be decided in a court of law." ;
    rdfs:comment "A class representing a Case" .
	

	
lexlegal:Article
    a owl:Class ;    
    rdfs:subClassOf lexlegal:Document;
    rdfs:subClassOf schema:Article;
    rdfs:isDefinedBy lexlegal: ;
    rdfs:label "Article" ;
 	dc:identifier "Article" ;
	dct:description "A piece of writing included with others in a newspaper, magazine, or other publication." ;
    rdfs:comment "A class representing a Legal Article" .
	

lexlegal:Citation
    a owl:Class ;    
    rdfs:subClassOf lexlegal:Document;
    rdfs:isDefinedBy lexlegal: ;
    rdfs:label "Citation" ;
 	dc:identifier "Citation" ;
	dct:description "A reference to a previous case, used as guidance in the trying of comparable cases or in support of an argument." ;
    rdfs:comment "A class representing a citation or cite " .
	

	
lexlegal:Statute
    a owl:Class ;    
    rdfs:subClassOf lexlegal:Document;
    rdfs:isDefinedBy lexlegal: ;
    rdfs:label "Statute" ;
 	dc:identifier "Statute" ;
	dct:description "A statute is a formal written enactment of a legislative authority that governs the legal entities of a city, state, or country by way of consent." ;
    rdfs:comment "A class representing a Statute " .
	

	
lexlegal:Legislation
    a owl:Class ;    
    rdfs:subClassOf lexlegal:Document;
    rdfs:subClassOf schema:Legislation;
    rdfs:isDefinedBy lexlegal: ;
    rdfs:label "Legislation" ;
 	dc:identifier "Legislation" ;
	dct:description "Laws, considered collectively" ;
    rdfs:comment "A class representing a Legislation" .
	

	
lexlegal:Constitution
    a owl:Class ;    
    rdfs:subClassOf lexlegal:Document;
    rdfs:isDefinedBy lexlegal: ;
    rdfs:label "Constitution" ;
 	dc:identifier "Constitution" ;
	dct:description "A body of fundamental principles or established precedents according to which a state or other organization is acknowledged to be governed" ;
    rdfs:comment "A class representing the Constitution" .
	

	
lexlegal:User
    a owl:Class ;    
    rdfs:subClassOf lexlegal:Person;
    rdfs:isDefinedBy lexlegal: ;
    rdfs:label "User" ;
 	dc:identifier "User" ;
	dct:description "A person who uses or operates Lexanalytics" ;
    rdfs:comment "A class representing a User" .
	

	
	
lexlegal:Organization
    a owl:Class;
    rdfs:subClassOf lexlegal:Object;
    rdfs:isDefinedBy lexlegal: ;
    rdfs:subClassOf foaf:Organization ;
	rdfs:subClassOf schema:Organization ;
    rdfs:label "Organization" ;
 	dc:identifier "Organization" ;
	dct:description "An organized group of people with a particular purpose, such as a business or government department." ;
    rdfs:comment "A class representing an Organization" .
	

	

lexlegal:Event
    a owl:Class ;
    rdfs:subClassOf lexlegal:Object;
    rdfs:subClassOf schema:Event;
	rdfs:isDefinedBy lexlegal: ;
    rdfs:label "Event" ;
 	dc:identifier "Event" ;
	dct:description "A thing that happens or takes place, especially one of importance." ;
    rdfs:comment "A class representing an Event" .

    
lexlegal:SearchEvent
    a owl:Class ;
    rdfs:subClassOf lexlegal:Event;
	rdfs:subClassOf schema:SearchAction ;
	rdfs:isDefinedBy lexlegal: ;
    rdfs:label "SearchEvent" ;
 	dc:identifier "SearchEvent" ;
	dct:description "todo" ;
    rdfs:comment "A class representing a Search Event" .
    


lexlegal:ViewEvent
    a owl:Class ;
    rdfs:subClassOf lexlegal:Event;
	rdfs:isDefinedBy lexlegal: ;
    rdfs:label "ViewEvent" ;
 	dc:identifier "ViewEvent" ;
	dct:description "todo" ;
    rdfs:comment "A class representing a Entity viewing Event" .
    


	
	
lexlegal:ItemData
    a owl:Class ;
    rdfs:subClassOf lexlegal:Object ;
    rdfs:subClassOf schema:DataFeed ;
    rdfs:isDefinedBy lexlegal: ;
    rdfs:label "ItemData" ;
 	dc:identifier "ItemData" ;
	dct:description "todo" ;
    rdfs:comment "Item Data" .
	
	
lexlegal:Subscription
    a owl:Class ;
    rdfs:subClassOf lexlegal:Object;
	rdfs:isDefinedBy lexlegal: ;
    rdfs:label "Subscription" ;
 	dc:identifier "Subscription" ;
	dct:description "An arrangement to receive something, typically a publication, regularly by paying in advance." ;
    rdfs:comment "A class representing a Subscription" .
    

lexlegal:Bookmark
    a owl:Class ;
    rdfs:subClassOf lexlegal:Object;
	rdfs:isDefinedBy lexlegal: ;
    rdfs:label "Bookmark" ;
 	dc:identifier "Bookmark" ;
	dct:description "A placeholder on a document to enable quick access in future" ;
    rdfs:comment "A class representing a Bookmark" .
    

lexlegal:Annotation
    a owl:Class ;
    rdfs:subClassOf lexlegal:Object;
	rdfs:isDefinedBy lexlegal: ;
    rdfs:label "Annotation" ;
 	dc:identifier "Annotation" ;
	dct:description "A note by way of explanation or comment added to a text " ;
    rdfs:comment "A class representing an Annotation" .
    

	
lexlegal:Judge
    a owl:Class ;    
    rdfs:subClassOf lexlegal:Person;
    rdfs:isDefinedBy lexlegal: ;
    rdfs:label "Judge" ;
 	dc:identifier "Judge" ;
	dct:description "A public officer appointed to decide cases in a law court." ;
    rdfs:comment "A class representing a Judge" .
	

lexlegal:Counsel
    a owl:Class ;    
    rdfs:subClassOf lexlegal:Person;
	rdfs:subClassOf schema:LegalService ;
    rdfs:isDefinedBy lexlegal: ;
    rdfs:label "Counsel" ;
 	dc:identifier "Counsel" ;
	dct:description "A legal counsel refers to a practitioner of law (an attorney or lawyer) who is allowed to practice in all courts of law" ;
    rdfs:comment "A class representing a Legal Counsel" .
	


lexlegal:Court
    a owl:Class;
    rdfs:isDefinedBy lexlegal: ;
    rdfs:subClassOf lexlegal:Organization ;
    rdfs:subClassOf schema:Courthouse ;
    rdfs:label "Court" ;
 	dc:identifier "Court" ;
	dct:description "A body of people presided over by a judge, judges, or magistrate, and acting as a tribunal in civil and criminal cases" ;
    rdfs:comment "A class representing a Court" .


lexlegal:File
    a owl:Class;
    rdfs:isDefinedBy lexlegal: ;
    rdfs:subClassOf lexlegal:Object ;
    rdfs:subClassOf schema:MediaObject ;
    rdfs:label "File" ;
 	dc:identifier "File" ;
	dct:description "A class representing a file such as an image, video, or audio object embedded in a web page or a downloadable dataset" ;
    rdfs:comment "A class representing a file such as an image, video, or audio object embedded in a web page or a downloadable dataset" .



# ---------------------------------------------------------------------------
# PROPERTIES
#


lexlegal:hasID
	rdf:type owl:DatatypeProperty, owl:InverseFunctionalProperty ;
	owl:equivalentProperty schema:identifier ;
	rdfs:isDefinedBy lexlegal: ;
	rdfs:label "hasID" ;
	dct:description "todo" ;
  	rdfs:comment "This property associates an instance of an Object with an Identity code" ;
 	rdfs:range xsd:string .


lexlegal:hasRef
	rdf:type owl:DatatypeProperty, owl:InverseFunctionalProperty ;
	owl:equivalentProperty schema:identifier ;
	rdfs:isDefinedBy lexlegal: ;
	rdfs:label "hasRef" ;
	dct:description "todo" ;
  	rdfs:comment "This property associates an instance of an Object with a Reference code" ;
	rdfs:range xsd:string .


lexlegal:hasSuitNumber
	rdf:type owl:DatatypeProperty, owl:InverseFunctionalProperty ;
	rdfs:subPropertyOf lexlegal:hasRef ;
	rdfs:isDefinedBy lexlegal: ;
	rdfs:label "hasSuitNumber" ;
	dct:description "todo" ;
  	rdfs:comment "This property associates an instance of a Case with a Suit Number" ;
	rdfs:domain lexlegal:Case ;
	rdfs:range xsd:string .


lexlegal:hasFirstName
	rdf:type owl:DatatypeProperty ;
	rdfs:subPropertyOf lexlegal:hasName ;
	rdfs:isDefinedBy lexlegal: ;
	rdfs:label "hasFirstName" ;
	dct:description "todo" ;
  	rdfs:comment "This property associates an instance of a Person Object with a First Name" ;
	rdfs:domain lexlegal:Person ;
	rdfs:range xsd:string .


lexlegal:hasLastName
	rdf:type owl:DatatypeProperty ;
	rdfs:subPropertyOf lexlegal:hasName ;
	rdfs:isDefinedBy lexlegal: ;
	rdfs:label "hasLastName" ;
	dct:description "todo" ;
  	rdfs:comment "This property associates an instance of a Person Object with a Last Name" ;
	rdfs:domain lexlegal:Person ;
	rdfs:range xsd:string .

	
lexlegal:hasURL
	rdf:type owl:ObjectProperty ;
	rdfs:subPropertyOf schema:url ;
	rdfs:subPropertyOf vcard:url ;
	rdfs:isDefinedBy lexlegal: ;
	rdfs:label "hasURL" ;
	dct:description "todo" ;
  	rdfs:comment "This property associates an instance of an Object with a URL" ;
	rdfs:range xsd:anyURI .

	
lexlegal:hasURI
	rdf:type owl:ObjectProperty ;
	rdfs:subPropertyOf schema:url ;
	rdfs:subPropertyOf vcard:url ;
	rdfs:isDefinedBy lexlegal: ;
	rdfs:label "hasURI" ;
	dct:description "todo" ;
  	rdfs:comment "This property associates an instance of an Object with a URI" ;
	rdfs:range xsd:anyURI .

	
lexlegal:hasMember
	rdf:type owl:ObjectProperty ;
	rdfs:subPropertyOf schema:memberOf ;
	rdfs:isDefinedBy lexlegal: ;
	rdfs:label "hasMember" ;
	dct:description "hasMember" ;
  	rdfs:comment "This property associates an instance of an Object with a member" ;
	rdfs:range lexlegal:Person .


lexlegal:isMemberOf
	  rdf:type owl:ObjectProperty ;
	  owl:inverseOf lexlegal:hasMember ;
	  rdfs:label "isMemberOf" ;
	  rdfs:comment "This property associates an instance of a Person with an Entity" ;
	  dct:description "todo" ;
	  rdfs:isDefinedBy lexlegal: ;
	  rdfs:domain lexlegal:Person .
  

  
 
	
lexlegal:hasEmail
	rdf:type owl:DatatypeProperty ;
	rdfs:subPropertyOf schema:email ;
	rdfs:isDefinedBy lexlegal: ;
	rdfs:label "hasEmail" ;
	dct:description "todo" ;
  	rdfs:comment "This property associates an instance of an Object with an Email" ;
	rdfs:range xsd:string .

	
lexlegal:hasPhone
	rdf:type owl:DatatypeProperty ;
	rdfs:subPropertyOf schema:telephone ;
	rdfs:isDefinedBy lexlegal: ;
	rdfs:label "hasPhone" ;
	dct:description "todo" ;
  	rdfs:comment "This property associates an instance of an Object with an Phone" ;
	rdfs:range xsd:string .

	
lexlegal:hasStartDate
	rdf:type owl:DatatypeProperty ;
	rdfs:subPropertyOf lexlegal:hasDate ;
	rdfs:isDefinedBy lexlegal: ;
	rdfs:label "hasStartDate" ;
	dct:description "todo" ;
	rdfs:comment "This property associates an instance of an Subscription Event with a Date" ;
	rdfs:domain lexlegal:Subscription ;
	rdfs:range xsd:date .

	
lexlegal:hasEndDate
	rdf:type owl:DatatypeProperty ;
	rdfs:subPropertyOf lexlegal:hasDate ;
	rdfs:isDefinedBy lexlegal: ;
	rdfs:label "hasEndDate" ;
	dct:description "todo" ;
	rdfs:comment "This property associates an instance of an Subscription Event with a Date" ;
	rdfs:domain lexlegal:Subscription ;
	rdfs:range xsd:date .



lexlegal:hasDuration
	rdf:type owl:DatatypeProperty ;
	rdfs:isDefinedBy lexlegal: ;
	rdfs:label "hasDuration" ;
	dct:description "todo" ;
	rdfs:comment "This property associates an instance of an Subscription Event with a Duration" ;
	rdfs:domain lexlegal:Subscription ;
	rdfs:range xsd:string .


lexlegal:hasDate
	rdf:type owl:DatatypeProperty ;
	owl:equivalentProperty dbo:eventDate ;
	rdfs:isDefinedBy lexlegal: ;
	dct:description "todo" ;
	rdfs:label "hasDate" ;
	rdfs:comment "This property associates an instance of an Event with a Date" ;
	rdfs:range xsd:date .

	
	
lexlegal:hasName
	rdf:type owl:DatatypeProperty ;
	rdfs:subPropertyOf schema:name ;
	rdfs:subPropertyOf dbo:name ;
	rdfs:subPropertyOf foaf:name ;
	rdfs:isDefinedBy lexlegal: ;
	rdfs:label "hasName" ;
	dct:description "todo" ;
  	rdfs:comment "This property associates an instance of an Object with a Name" ;
	rdfs:range xsd:string .

	
lexlegal:hasCount
	rdf:type owl:DatatypeProperty ;
	rdfs:isDefinedBy lexlegal: ;
	rdfs:label "hasCount" ;
	rdfs:comment "This property associates an instance of an Object with a number" ;
	dct:description "todo" ;
	rdfs:range xsd:double .



lexlegal:hasDocumentType
	rdf:type owl:DatatypeProperty ;
	rdfs:isDefinedBy lexlegal: ;
	rdfs:label "hasDocumentType" ;
	dct:description "todo" ;
	rdfs:comment "This property associates an instance of an Object with a Document Type" ;
	rdfs:range xsd:string .



lexlegal:hasContent
	rdf:type owl:DatatypeProperty ;
	rdfs:isDefinedBy lexlegal: ;
	rdfs:label "hasContent" ;
	dct:description "todo" ;
	rdfs:comment "This property associates an instance of an Object with a Content" ;
	rdfs:range xsd:string .


lexlegal:hasAbstract
	rdf:type owl:DatatypeProperty ;
	rdfs:isDefinedBy lexlegal: ;
	rdfs:label "hasAbstract" ;
	rdfs:comment "This property associates an instance of an Object with an Abstract Content" ;
	dct:description "todo" ;
	rdfs:range xsd:string .


lexlegal:hasLocation
	  rdf:type owl:DatatypeProperty ;
	  rdfs:label "hasLocation" ;
	  dct:description "todo" ;
	  rdfs:comment "This property associates an instance of an Object with an Address" ;
	  rdfs:isDefinedBy lexlegal: ;
	  rdfs:range xsd:anyURI .

	  
lexlegal:isSectorOf
	  rdf:type owl:DatatypeProperty ;
	  rdfs:label "isSectorOf" ;
	  rdfs:comment "This property associates an instance of an Object with a Sector" ;
	  dct:description "todo" ;
	  rdfs:isDefinedBy lexlegal: ;
	  rdfs:range xsd:string .
  

lexlegal:hasOrganization
	  rdf:type owl:DatatypeProperty ;
	  rdfs:label "hasOrganization" ;
	  dct:description "todo" ;
	  rdfs:comment "This property associates an instance of a Case with a Organization" ;
	  rdfs:isDefinedBy lexlegal: ;
	  rdfs:domain lexlegal:Case ;
	  rdfs:range lexlegal:Organization.
  


  
lexlegal:hasTitle
	  rdf:type owl:DatatypeProperty ;
	  rdfs:label "hasTitle" ;
	  dct:description "todo" ;
	  rdfs:comment "This property associates an instance of an Object with a Title" ;
	  rdfs:isDefinedBy lexlegal: ;
	  rdfs:range xsd:string .
  


lexlegal:hasVerdict
	  rdf:type owl:DatatypeProperty ;
	  rdfs:label "hasVerdict" ;
	  rdfs:comment "This property associates an instance of an Object with a verdict" ;
	  dct:description "todo" ;
	  rdfs:isDefinedBy lexlegal: ;
	  rdfs:domain lexlegal:Case ;
	  rdfs:range xsd:string .
  


lexlegal:hasAppeal
	  rdf:type owl:DatatypeProperty ;
	  rdfs:label "hasAppeal" ;
	  rdfs:comment "This property associates an instance of an Object with an appeal note" ;
	  dct:description "todo" ;
	  rdfs:isDefinedBy lexlegal: ;
	  rdfs:domain lexlegal:Case ;
	  rdfs:range xsd:string .
  


lexlegal:hasDateDecided
	  rdf:type owl:DatatypeProperty ;
	  rdfs:subPropertyOf lexlegal:hasDate ;
	  rdfs:label "hasDateDecided" ;
	  rdfs:comment "This property associates an instance of a Case with the date it was decided" ;
	  dct:description "todo" ;
	  rdfs:isDefinedBy lexlegal: ;
	  rdfs:domain lexlegal:Case ;
	  rdfs:range xsd:string . 
  


lexlegal:hasDeliveredJudgement 
	  rdf:type owl:DatatypeProperty ;
	  rdfs:label "hasDeliveredJudgement" ;
	  rdfs:comment "This property associates an instance of a Case with a Delivered Judgement" ;
	  dct:description "todo" ;
	  rdfs:isDefinedBy lexlegal: ;
	  rdfs:domain lexlegal:Case ;
	  rdfs:range xsd:string .
  


lexlegal:hasCounsel
	  rdf:type owl:DatatypeProperty ;
	  rdfs:label "hasCounsel" ;
	  rdfs:comment "This property associates an instance of a Case with a Counsel" ;
	  dct:description "todo" ;
	  rdfs:isDefinedBy lexlegal: ;
	  rdfs:domain lexlegal:Case ;
	  rdfs:range lexlegal:Counsel .
  


lexlegal:hasCounselAppellant
	  rdf:type owl:DatatypeProperty ;
	  rdfs:subPropertyOf lexlegal:hasCounsel ;
	  rdfs:label "hasCounselAppellant" ;
	  rdfs:comment "This property associates an instance of a Case with a Counsel for the Appellant" ;
	  dct:description "todo" ;
	  rdfs:isDefinedBy lexlegal: ;
	  rdfs:domain lexlegal:Case ;
	  rdfs:range lexlegal:Counsel .
  

lexlegal:hasCounselRespondent
	  rdf:type owl:DatatypeProperty ;
	  rdfs:subPropertyOf lexlegal:hasCounsel ;
	  rdfs:label "hasCounselRespondent" ;
	  rdfs:comment "This property associates an instance of a Case with a Counsel for the Respondent" ;
	  dct:description "todo" ;
	  rdfs:isDefinedBy lexlegal: ;
	  rdfs:domain lexlegal:Case ;
	  rdfs:range lexlegal:Counsel .
  


  

lexlegal:hasCauseOfAction
	  rdf:type owl:DatatypeProperty ;
	  rdfs:label "hasCauseOfAction" ;
	  rdfs:comment "This property associates an instance of a Case with a Cause of Action eg fraud breach of contract etc" ;
	  dct:description "todo" ;
	  rdfs:isDefinedBy lexlegal: ;
	  rdfs:domain lexlegal:Case ;
	  rdfs:seeAlso p:Cause_of_action ;
	  rdfs:range xsd:string .
  


lexlegal:hasMotionType
	  rdf:type owl:DatatypeProperty ;
	  rdfs:label "hasMotionType" ;
	  rdfs:comment "This property associates an instance of a Case with a motion type" ;
	  dct:description "todo" ;
	  rdfs:isDefinedBy lexlegal: ;
	  rdfs:domain lexlegal:Case ;
	  rdfs:range xsd:string .
  


lexlegal:hasAppelant
	  rdf:type owl:DatatypeProperty ;
	  rdfs:label "hasAppelant" ;
	  rdfs:comment "This property associates an instance of a Case with who is appealing the judgement before the court" ;
	  dct:description "todo" ;
	  rdfs:isDefinedBy lexlegal: ;
	  rdfs:domain lexlegal:Case ;
	  rdfs:range xsd:string .
  


lexlegal:hasRespondent
	  rdf:type owl:DatatypeProperty ;
	  rdfs:label "hasRespondent" ;
	  rdfs:comment "This property associates an instance of a Case with who is required to answer for a petition brought before the court" ;
	  dct:description "todo" ;
	  rdfs:isDefinedBy lexlegal: ;
	  rdfs:domain lexlegal:Case ;
	  rdfs:range xsd:string .
  

 
lexlegal:hasIssue
	  rdf:type owl:DatatypeProperty ;
	  rdfs:label "hasIssue" ;
	  rdfs:comment "This property associates an instance of an Case with an issue" ;
	  dct:description "todo" ;
	  rdfs:isDefinedBy lexlegal: ;
	  rdfs:domain lexlegal:Case ;
	  rdfs:range xsd:string .
  


lexlegal:hasFact
	  rdf:type owl:DatatypeProperty ;
	  rdfs:label "hasFact" ;
	  rdfs:comment "This property associates an instance of a Case with a fact" ;
	  dct:description "todo" ;
	  rdfs:isDefinedBy lexlegal: ;
	  rdfs:domain lexlegal:Case ;
	  rdfs:range xsd:string .
  

lexlegal:hasFactWordFreq
	  rdf:type owl:DatatypeProperty ;
	  rdfs:label "hasFactWordFreq" ;
	  rdfs:comment "This property associates Word Frequencies to the Fact of a Case" ;
	  dct:description "todo" ;
	  rdfs:isDefinedBy lexlegal: ;
	  rdfs:domain lexlegal:Case ;
	  rdfs:range xsd:string .
  

lexlegal:hasFactEntities
	  rdf:type owl:DatatypeProperty ;
	  rdfs:label "hasFactEntities" ;
	  rdfs:comment "This property associates Entities to the Fact of a Case" ;
	  dct:description "todo" ;
	  rdfs:isDefinedBy lexlegal: ;
	  rdfs:domain lexlegal:Case ;
	  rdfs:range xsd:string .
  

lexlegal:hasFactTopics
	  rdf:type owl:DatatypeProperty ;
	  rdfs:label "hasFactTopics" ;
	  rdfs:comment "This property associates Topics to the Fact of a Case" ;
	  dct:description "todo" ;
	  rdfs:isDefinedBy lexlegal: ;
	  rdfs:domain lexlegal:Case ;
	  rdfs:range xsd:string .
  



lexlegal:hasPrinciples
	  rdf:type owl:DatatypeProperty ;
	  rdfs:label "hasPrinciples" ;
	  rdfs:comment "This property associates an instance of a Case with principles" ;
	  dct:description "todo" ;
	  rdfs:isDefinedBy lexlegal: ;
	  rdfs:domain lexlegal:Case ;
	  rdfs:range xsd:string .
  


lexlegal:hasSubjectMatter
	  rdf:type owl:DatatypeProperty ;
	  rdfs:label "hasSubjectMatter" ;
	  rdfs:comment "This property associates an instance of a Case with a subject matter of law treated in the case" ;
	  dct:description "todo" ;
	  rdfs:isDefinedBy lexlegal: ;
	  rdfs:domain lexlegal:Case ;
	  rdfs:range xsd:string .
  


lexlegal:hasCaseHistory
	  rdf:type owl:DatatypeProperty ;
	  rdfs:label "hasCaseHistory" ;
	  rdfs:comment "This property associates an instance of a Case with a case history" ;
	  dct:description "todo" ;
	  rdfs:isDefinedBy lexlegal: ;
	  rdfs:domain lexlegal:Case ;
	  rdfs:range xsd:string .

	  
lexlegal:hasForeignCourtRulesReferred
	  rdf:type owl:DatatypeProperty ;
	  rdfs:label "hasForeignCourtRulesReferred" ;
	  rdfs:comment "This property associates an instance of a Case with a foreign court rule that were referred to or cited in the judgement" ;
	  dct:description "todo" ;
	  rdfs:isDefinedBy lexlegal: ;
	  rdfs:domain lexlegal:Case ;
	  rdfs:range xsd:string .
  


  
lexlegal:hasReferredForeignCase
	  rdf:type owl:ObjectProperty ;
	  rdfs:subPropertyOf lexlegal:hasReferredCase ;
	  rdfs:label "hasReferredForeignCase" ;
	  rdfs:comment "This property associates an instance of a Case with a Foreign case that were referred to or cited in the judgement" ;
	  dct:description "todo" ;
	  rdfs:isDefinedBy lexlegal: ;
	  rdfs:domain lexlegal:Case ;
	  rdfs:range lexlegal:Case .
  

lexlegal:hasReferredLocalCase
	  rdf:type owl:ObjectProperty ;
	  rdfs:subPropertyOf lexlegal:hasReferredCase ;
	  rdfs:label "hasReferredLocalCase" ;
	  rdfs:comment "This property associates an instance of a Case with a Local case that were referred to or cited in the judgement" ;
	  dct:description "todo" ;
	  rdfs:isDefinedBy lexlegal: ;
	  rdfs:domain lexlegal:Case ;
	  rdfs:range lexlegal:Case .
  

lexlegal:hasReferredCase
	  rdf:type owl:ObjectProperty ;
	  rdfs:label "hasReferredCase" ;
	  rdfs:comment "This property associates an instance of a Case with a case that were referred to or cited in the judgement" ;
	  dct:description "todo" ;
	  rdfs:isDefinedBy lexlegal: ;
	  rdfs:domain lexlegal:Case ;
	  rdfs:range lexlegal:Case .
  

lexlegal:wasReferrencedBy
	  rdf:type owl:ObjectProperty ;
	  owl:inverseOf lexlegal:hasReferredCase ;
	  rdfs:label "wasReferrencedBy" ;
	  rdfs:comment "This property associates an instance of a Case with a case that referenced or referred it" ;
	  dct:description "todo" ;
	  rdfs:isDefinedBy lexlegal: ;
	  rdfs:domain lexlegal:Case ;
	  rdfs:range lexlegal:Case .
  

lexlegal:hasStatute
	  rdf:type owl:DatatypeProperty ;
	  rdfs:label "hasStatute" ;
	  rdfs:comment "This property associates an instance of a Case with a statute that were referred to or cited in the judgement" ;
	  dct:description "todo" ;
	  rdfs:isDefinedBy lexlegal: ;
	  rdfs:domain lexlegal:Case ;
	  rdfs:range xsd:string .
  


lexlegal:hasReferredStatute
	  rdf:type owl:DatatypeProperty ;
	  rdfs:subPropertyOf lexlegal:hasStatute ;
	  rdfs:label "hasReferredStatute" ;
	  rdfs:comment "This property associates an instance of a Case with a Local statute that were referred to or cited in the judgement" ;
	  dct:description "todo" ;
	  rdfs:isDefinedBy lexlegal: ;
	  rdfs:domain lexlegal:Case ;
	  rdfs:range xsd:string .
  

lexlegal:hasReferredForeignStatute
	  rdf:type owl:DatatypeProperty ;
	  rdfs:subPropertyOf lexlegal:hasStatute ;
	  rdfs:label "hasReferredForeignStatute" ;
	  rdfs:comment "This property associates an instance of a Case with a Foreign statute that were referred to or cited in the judgement" ;
	  dct:description "todo" ;
	  rdfs:isDefinedBy lexlegal: ;
	  rdfs:domain lexlegal:Case ;
	  rdfs:range xsd:string .
  

lexlegal:hasCourt
	  rdf:type owl:ObjectProperty ;
	  rdfs:label "hasCourt" ;
	  rdfs:comment "This property associates an instance of a Case with a court type " ;
	  dct:description "todo" ;
	  rdfs:isDefinedBy lexlegal: ;
	  rdfs:domain lexlegal:Case ;
	  rdfs:range lexvocab:CourtType .
  

lexlegal:hasJudge
	  rdf:type owl:ObjectProperty ;
	  rdfs:label "hasJudge" ;
	  rdfs:comment "This property associates an instance of a case with a Judge" ;
	  dct:description "todo" ;
	  rdfs:isDefinedBy lexlegal: ;
	  rdfs:domain lexlegal:Judge ;
	  rdfs:range lexlegal:Case .
  

 
lexlegal:hasOtherJudge
	  rdf:type owl:ObjectProperty ;
	  rdfs:subPropertyOf lexlegal:hasJudge ;
	  rdfs:label "hasOtherJudge" ;
	  rdfs:comment "This property associates an instance of a Case with an unclassified judge " ;
	  dct:description "todo" ;
	  rdfs:isDefinedBy lexlegal: ;
	  rdfs:domain lexlegal:Case ;
	  rdfs:range lexlegal:Judge .
  

lexlegal:hasJudgeWithConcurringOpinion
	  rdf:type owl:ObjectProperty ;
	  rdfs:subPropertyOf lexlegal:hasJudge ;
	  rdfs:label "hasJudgeWithConcurringOpinion" ;
	  rdfs:comment "This property associates an instance of a Case with a judge that agrees with the decision made by majority of the court" ;
	  dct:description "todo" ;
	  rdfs:isDefinedBy lexlegal: ;
	  rdfs:domain lexlegal:Case ;
	  rdfs:range lexlegal:Judge .
  

lexlegal:hasJudgeWithDissent
	  rdf:type owl:ObjectProperty ;
	  rdfs:subPropertyOf lexlegal:hasJudge ;
	  rdfs:label "hasJudgeWithDissent" ;
	  rdfs:comment "This property associates an instance of a Case with the judge that delivered dissenting opinion" ;
	  dct:description "todo" ;
	  rdfs:isDefinedBy lexlegal: ;
	  rdfs:domain lexlegal:Case ;
	  rdfs:range lexlegal:Judge .
  

lexlegal:hasJudgeMajorityJudgement
	  rdf:type owl:ObjectProperty ;
	  rdfs:subPropertyOf lexlegal:hasJudge ;
	  rdfs:label "hasJudgeMajorityJudgement" ;
	  rdfs:comment "This property associates an instance of a Case with the judge that delivered leading judgement" ;
	  dct:description "todo" ;
	  rdfs:isDefinedBy lexlegal: ;
	  rdfs:domain lexlegal:Case ;
	  rdfs:range lexlegal:Judge .
  

lexlegal:hasPresidingJudge
	  rdf:type owl:ObjectProperty ;
	  rdfs:subPropertyOf lexlegal:hasJudge ;
	  rdfs:label "hasPresidingJudge" ;
	  rdfs:comment "This property associates an instance of a Case with the judge that presided over the case" ;
	  owl:equivalentProperty lexlegal:hasJudgeMajorityJudgement, lexlegal:hasJudgeWithDissent, lexlegal:hasJudgeWithConcurringOpinion, lexlegal:hasOtherJudges ;
	  dct:description "todo" ;
	  rdfs:isDefinedBy lexlegal: ;
	  rdfs:domain lexlegal:Case ;
	  rdfs:range lexlegal:Judge .
  

  
lexlegal:isJudgeOf
	  rdf:type owl:ObjectProperty ;
	  owl:inverseOf lexlegal:hasJudge ;
	  rdfs:label "isJudgeOf" ;
	  rdfs:comment "This property associates an instance of a Judge with a case" ;
	  dct:description "todo" ;
	  rdfs:isDefinedBy lexlegal: ;
	  rdfs:domain lexlegal:Judge ;
	  rdfs:range lexlegal:Case .
  

  
  
  
  

lexlegal:hasAuthor
	  rdf:type owl:DatatypeProperty ;
	  rdfs:subPropertyOf schema:author ;
	  rdfs:label "hasAuthor" ;
	  rdfs:comment "This property associates an instance of an Object with an Author" ;
	  dct:description "todo" ;
	  rdfs:isDefinedBy lexlegal: ;
	  rdfs:domain lexlegal:Article ;
	  rdfs:range xsd:string .
  


lexlegal:isAuthorOf
	  rdf:type owl:ObjectProperty ;
	  owl:inverseOf lexlegal:hasAuthor ;
	  rdfs:label "isAuthorOf" ;
	  rdfs:comment "This property associates an instance of an Object with an Article" ;
	  dct:description "todo" ;
	  rdfs:isDefinedBy lexlegal: ;
	  rdfs:domain lexlegal:Person ;
	  rdfs:range lexlegal:Article .
  


lexlegal:hasAreaOfLaw
	  rdf:type owl:ObjectProperty ;
	  rdfs:label "hasAreaOfLaw" ;
	  rdfs:comment "This property associates an instance of an Article or a Case with an Area of Law" ;
	  dct:description "todo" ;
	  rdfs:isDefinedBy lexlegal: ;
	  rdfs:domain lexlegal:Article, lexlegal:Case ;
	  rdfs:range lexvocab:AreaOfLaw .
  


lexlegal:hasCitation
	  rdf:type owl:ObjectProperty ;
	  rdfs:subPropertyOf schema:citation ;
	  rdfs:label "hasCitation" ;
	  rdfs:comment "This property associates an instance of a Document with a Citation" ;
	  dct:description "todo" ;
	  rdfs:isDefinedBy lexlegal: ;
	  rdfs:domain lexlegal:Article, lexlegal:Case ;
	  rdfs:range lexlegal:Citation .


lexlegal:citedBy
	  rdf:type owl:ObjectProperty ;
	  owl:inverseOf lexlegal:hasCitation ;
	  rdfs:subPropertyOf schema:citation ;
	  rdfs:label "citedBy" ;
	  rdfs:comment "This property associates an instance of a Citation with a Document" ;
	  dct:description "todo" ;
	  rdfs:isDefinedBy lexlegal: .
	  

lexlegal:hasReferredCitation
	  rdf:type owl:ObjectProperty ;
	  rdfs:subPropertyOf schema:citation ;
	  rdfs:label "hasCitation" ;
	  rdfs:comment "This property associates an instance of a Document with a referred Citation" ;
	  dct:description "todo" ;
	  rdfs:isDefinedBy lexlegal: ;
	  rdfs:domain lexlegal:Article, lexlegal:Case ;
	  rdfs:range lexlegal:Citation .



lexlegal:hasParty
	  rdf:type owl:ObjectProperty ;
	  rdfs:label "hasParty" ;
	  rdfs:comment "This property associates an instance of a Document with a Party or Person" ;
	  dct:description "todo" ;
	  rdfs:isDefinedBy lexlegal: ;
	  rdfs:domain lexlegal:Case ;
	  rdfs:range lexlegal:Person .
  

lexlegal:isPartyOf
	  rdf:type owl:ObjectProperty ;
	  rdfs:label "isPartyOf" ;
	  owl:inverseOf lexlegal:hasParty ;
	  rdfs:comment "This property associates an instance of a Party or Person with a Document" ;
	  dct:description "todo" ;
	  rdfs:isDefinedBy lexlegal: .
  


lexlegal:hasDefendant
	  rdf:type owl:ObjectProperty ;
	  rdfs:subPropertyOf lexlegal:hasParty ;
	  rdfs:label "hasDefendant" ;
	  rdfs:comment "This property associates a Case with a Defendant" ;
	  dct:description "todo" ;
	  rdfs:isDefinedBy lexlegal: ;
	  rdfs:domain lexlegal:Case ;
	  rdfs:range lexlegal:Person .
  

  
lexlegal:hasPlantiff
	  rdf:type owl:ObjectProperty ;
	  rdfs:subPropertyOf lexlegal:hasParty ;
	  rdfs:label "hasPlantiff" ;
	  rdfs:comment "This property associates a Case with a Plantiff" ;
	  dct:description "todo" ;
	  rdfs:isDefinedBy lexlegal: ;
	  rdfs:domain lexlegal:Case ;
	  rdfs:range lexlegal:Person .
  

lexlegal:hasAppellant
	  rdf:type owl:ObjectProperty ;
	  rdfs:subPropertyOf lexlegal:hasParty ;
	  rdfs:label "hasAppellant" ;
	  rdfs:comment "This property associates a Case with an Appellant" ;
	  dct:description "todo" ;
	  rdfs:isDefinedBy lexlegal: ;
	  rdfs:domain lexlegal:Case ;
	  rdfs:range lexlegal:Person .
  

lexlegal:hasRespondent
	  rdf:type owl:ObjectProperty ;
	  rdfs:subPropertyOf lexlegal:hasParty ;
	  rdfs:label "hasRespondent" ;
	  rdfs:comment "This property associates a Case with a Respondent" ;
	  dct:description "todo" ;
	  rdfs:isDefinedBy lexlegal: ;
	  rdfs:domain lexlegal:Case ;
	  rdfs:range lexlegal:Person .
  

  
lexlegal:hasJudgement
	  rdf:type owl:DatatypeProperty ;
	  rdfs:label "hasJudgement" ;
	  rdfs:comment "This property associates an instance of a Case with a Judgement" ;
	  dct:description "todo" ;
	  rdfs:isDefinedBy lexlegal: ;
	  rdfs:domain lexlegal:Case ;
	  rdfs:range xsd:string .
  

  
lexlegal:hasCauseOfAction
	rdf:type owl:ObjectProperty ;
  	rdfs:label "hasCauseOfAction" ;
  	rdfs:comment "This property associates an instance of a Case with a cause of action" ;
	dct:description "todo" ;
    rdfs:isDefinedBy lexlegal: ;
  	rdfs:domain lexlegal:Case ;
  	rdfs:range lexvocab:CauseOfAction .


  
lexlegal:hasMotionType
	rdf:type owl:ObjectProperty ;
  	rdfs:label "hasMotionType" ;
  	rdfs:comment "This property associates an instance of a Case with a motion type" ;
	dct:description "todo" ;
    rdfs:isDefinedBy lexlegal: ;
  	rdfs:domain lexlegal:Case ;
  	rdfs:range lexvocab:MotionType .


  
lexlegal:hasPartyType
	rdf:type owl:ObjectProperty ;
  	rdfs:label "hasPartyType" ;
  	rdfs:comment "This property associates an instance of a Case with a party type" ;
    rdfs:isDefinedBy lexlegal: ;
	dct:description "todo" ;
  	rdfs:domain lexlegal:Case ;
  	rdfs:range lexvocab:PartyType .


  
lexlegal:isAbout
	  rdf:type owl:DatatypeProperty ;
	  rdfs:label "isAbout" ;
	  rdfs:comment "This property associates an instance of an Object with an About" ;
	  dct:description "todo" ;
	  rdfs:isDefinedBy lexlegal: ;
	  rdfs:range xsd:string .
	  
	  
  
lexlegal:hasTopic
	rdf:type owl:ObjectProperty ;
	rdfs:subPropertyOf dct:subject ;
  	rdfs:label "hasTopic" ;
  	rdfs:comment "This property associates an instance of a Legal Document with a Legal Topic" ;
    rdfs:isDefinedBy lexlegal: ;
	dct:description "todo" ;
  	rdfs:range lexvocab:LexanalyticsTerms .



# ---------------------------------------------------------------------------
# citation properties
#
  
lexlegal:hasVolume
	  rdf:type owl:DatatypeProperty ;
	  rdfs:label "hasVolume" ;
	  rdfs:comment "This property associates an instance of a Citation with a volume number of the reporter in which the case appears" ;
	  dct:description "todo" ;
	  rdfs:isDefinedBy lexlegal: ;
	  rdfs:domain lexlegal:Citation ;
	  rdfs:range xsd:string .
  

lexlegal:hasReporter
	  rdf:type owl:DatatypeProperty ;
	  rdfs:label "hasReporter" ;
	  rdfs:comment "This property associates an instance of a Citation with a reporter" ;
	  dct:description "todo" ;
	  rdfs:isDefinedBy lexlegal: ;
	  rdfs:domain lexlegal:Citation ;
	  rdfs:range xsd:string .
  

lexlegal:hasPage
	  rdf:type owl:DatatypeProperty ;
	  rdfs:label "hasPage" ;
	  rdfs:comment "This property associates an instance of a Citation with the page on which the case begins" ;
	  dct:description "todo" ;
	  rdfs:isDefinedBy lexlegal: ;
	  rdfs:domain lexlegal:Citation ;
	  rdfs:range xsd:string .
  

lexlegal:hasYear
	  rdf:type owl:DatatypeProperty ;
	  rdfs:label "hasYear" ;
	  rdfs:comment "This property associates an instance of a Citation with the year the decision was rendered" ;
	  dct:description "todo" ;
	  rdfs:isDefinedBy lexlegal: ;
	  rdfs:domain lexlegal:Citation ;
	  rdfs:range xsd:string .
  

  
lexlegal:hasCoverArea
	  rdf:type owl:ObjectProperty ;
	  rdfs:label "hasCoverArea" ;
	  rdfs:comment "This property associates a Statue with a geographic region" ;
	  dct:description "todo" ;
	  rdfs:isDefinedBy lexlegal: ;
	  rdfs:domain lexlegal:Statute ;
	  rdfs:range xsd:anyURI .
  
# ----- end citation
  
 
lexlegal:hasEntity
	  rdf:type owl:DatatypeProperty ;
	  rdfs:label "hasEntity" ;
	  rdfs:comment "This property associates an instance of an Object with a Mention of an Entity" ;
	  dct:description "todo" ;
	  rdfs:isDefinedBy lexlegal: ;
	  rdfs:range xsd:string .
  

  
  
lexlegal:wasViewed
	  rdf:type owl:DatatypeProperty ;
	  rdfs:label "wasViewed" ;
	  rdfs:comment "This property associates an instance of an Event with a document viewing" ;
	  dct:description "todo" ;
	  rdfs:isDefinedBy lexlegal: ;
	  rdfs:domain lexlegal:Event ;
	  rdfs:range xsd:string .
  
lexlegal:wasSearched
	  rdf:type owl:DatatypeProperty ;
	  rdfs:label "wasSearched" ;
	  rdfs:comment "This property associates an instance of an Event with a document search" ;
	  dct:description "todo" ;
	  rdfs:isDefinedBy lexlegal: ;
	  rdfs:domain lexlegal:Event ;
	  rdfs:range xsd:string .
  
lexlegal:isStemmerSynonym
	  rdf:type owl:DatatypeProperty ;
	  rdfs:label "isStemmerSynonym" ;
	  rdfs:comment "This property associates an altlabel with its stemmer" ;
	  dct:description "todo" ;
	  rdfs:isDefinedBy lexlegal: ;
	  rdfs:domain lexvocab:Concept ;
	  rdfs:range xsd:string .
  
lexlegal:hasFactTopicsStemmed
	  rdf:type owl:DatatypeProperty ;
	  rdfs:label "hasFactTopicsStemmed" ;
	  rdfs:comment "This property associates Stemmed Topics to the Fact of a Case" ;
	  dct:description "todo" ;
	  rdfs:isDefinedBy lexlegal: ;
	  rdfs:domain lexlegal:Case ;
	  rdfs:range xsd:string .
  

# 2022

lexlegal:hasDateDecided
	rdf:type owl:DatatypeProperty ;
	rdfs:subPropertyOf lexlegal:hasDate ;
	rdfs:isDefinedBy lexlegal: ;
	dct:description "Decided Date of a Case" ;
	rdfs:label "hasDateDecided" ;
	rdfs:comment "This property associates an instance of a Case with a Decided Date" ;
	rdfs:range xsd:date .


lexlegal:hasPracticeProcedureIssues
	  rdf:type owl:DatatypeProperty ;
	  rdfs:label "hasPracticeProcedureIssues" ;
	  rdfs:comment "This property associates an instance of a Case with Practice & Procedure Issues" ;
	  dct:description "Practice & Procedure Issues of a Case" ;
	  rdfs:isDefinedBy lexlegal: ;
	  rdfs:domain lexlegal:Case ;
	  rdfs:range xsd:string .
  

lexlegal:hasIssuesForDeterminationAppellant
	  rdf:type owl:DatatypeProperty ;
	  rdfs:label "hasIssuesForDeterminationAppellant" ;
	  rdfs:comment "This property associates an instance of a Case with Issues for Determination for Appellant" ;
	  dct:description "Issues for Determination Appellant" ;
	  rdfs:isDefinedBy lexlegal: ;
	  rdfs:domain lexlegal:Case ;
	  rdfs:range xsd:string .
  


lexlegal:hasIssuesForDeterminationRespondent
	  rdf:type owl:DatatypeProperty ;
	  rdfs:label "hasIssuesForDeterminationRespondent" ;
	  rdfs:comment "This property associates an instance of a Case with Issues for Determination for Respondent" ;
	  dct:description "Issues for Determination Respondent" ;
	  rdfs:isDefinedBy lexlegal: ;
	  rdfs:domain lexlegal:Case ;
	  rdfs:range xsd:string .
  


lexlegal:hasSummary
	  rdf:type owl:DatatypeProperty ;
	  rdfs:label "hasSummary" ;
	  rdfs:comment "This property associates an instance of a Case with a Summary" ;
	  dct:description "Case Summary" ;
	  rdfs:isDefinedBy lexlegal: ;
	  rdfs:domain lexlegal:Case ;
	  rdfs:range xsd:string .
  

lexlegal:hasNigerianConstitutionSection2011
	  rdf:type owl:ObjectProperty ;
	  rdfs:label "hasNigerianConstitutionSection2011" ;
	  rdfs:comment "This property associates an instance of a Case with a Section of the Nigerian Constitution" ;
	  dct:description "Section of 2011 Nigerian Constitution" ;
	  rdfs:isDefinedBy lexlegal: ;
	  rdfs:domain lexlegal:Case ;
	  rdfs:range lexlegal:Constitution .


lexlegal:hasWikiURI
	  rdf:type owl:ObjectProperty ;
	  rdfs:label "hasWikiURI" ;
	  dct:description "Wikipedia reference for this object" ;
	  rdfs:comment "This property associates an instance of an Object with a Wikipedia URI" ;
	  rdfs:isDefinedBy lexlegal: ;
	  rdfs:range xsd:anyURI .

	  
	